Second constraint generator: checking with a candidate type

theories/Stlc/Symbolic/FreeCheck.v
@@ -1,180 +1,466 @@
+(******************************************************************************)
+(* Copyright (c) 2023 Denis Carnier, Steven Keuchel                           *)
+(* All rights reserved.                                                       *)
+(*                                                                            *)
+(* Redistribution and use in source and binary forms, with or without         *)
+(* modification, are permitted provided that the following conditions are     *)
+(* met:                                                                       *)
+(*                                                                            *)
+(* 1. Redistributions of source code must retain the above copyright notice,  *)
+(*    this list of conditions and the following disclaimer.                   *)
+(*                                                                            *)
+(* 2. Redistributions in binary form must reproduce the above copyright       *)
+(*    notice, this list of conditions and the following disclaimer in the     *)
+(*    documentation and/or other materials provided with the distribution.    *)
+(*                                                                            *)
+(* THIS SOFTWARE IS PROVIDED BY THE COPYRIGHT HOLDERS AND CONTRIBUTORS        *)
+(* "AS IS" AND ANY EXPRESS OR IMPLIED WARRANTIES, INCLUDING, BUT NOT LIMITED  *)
+(* TO, THE IMPLIED WARRANTIES OF MERCHANTABILITY AND FITNESS FOR A PARTICULAR *)
+(* PURPOSE ARE DISCLAIMED. IN NO EVENT SHALL THE COPYRIGHT HOLDER OR          *)
+(* CONTRIBUTORS BE LIABLE FOR ANY DIRECT, INDIRECT, INCIDENTAL, SPECIAL,      *)
+(* EXEMPLARY, OR CONSEQUENTIAL DAMAGES (INCLUDING, BUT NOT LIMITED TO,        *)
+(* PROCUREMENT OF SUBSTITUTE GOODS OR SERVICES; LOSS OF USE, DATA, OR         *)
+(* PROFITS; OR BUSINESS INTERRUPTION) HOWEVER CAUSED AND ON ANY THEORY OF     *)
+(* LIABILITY, WHETHER IN CONTRACT, STRICT LIABILITY, OR TORT (INCLUDING       *)
+(* NEGLIGENCE OR OTHERWISE) ARISING IN ANY WAY OUT OF THE USE OF THIS         *)
+(* SOFTWARE, EVEN IF ADVISED OF THE POSSIBILITY OF SUCH DAMAGE.               *)
+(******************************************************************************)
 
-Module CandidateType.
+From Coq Require Import
+  Strings.String.
+From Equations Require Import
+  Equations.
+From stdpp Require Import
+  base gmap.
+From Em Require Import
+  Context
+  Environment
+  Prelude
+  Stlc.Alloc
+  Stlc.Instantiation
+  Stlc.Persistence
+  Stlc.Predicates
+  Stlc.Sem
+  Stlc.Spec
+  Stlc.Symbolic.Free
+  Stlc.Unification
+  Stlc.Worlds.
 
+Import ctx.notations.
+Import World.notations.
+
+Set Implicit Arguments.
+
+#[local] Notation "s [ ζ ]" :=
+  (persist s ζ)
+    (at level 8, left associativity,
+      format "s [ ζ ]").
+
+Section Generate.
+  Import MonadNotations.
   Import World.notations.
 
-  #[local] Set Implicit Arguments.
-  #[local] Arguments step : simpl never.
-
-  Section Check.
-    Import World.notations.
-
-    #[local] Notation "[ ω ] x <- ma ;; mb" :=
-      (bind (R := Alloc) ma (fun _ ω x => mb))
-        (at level 80, x at next level,
-          ma at next level, mb at level 200,
-          right associativity).
-
-    #[local] Notation "∃ n , m" :=
-      (Bind_Exists_Free _ _ n m)
-        (at level 80, right associativity, format "∃ n ,  m").
-
-    #[local] Notation "t1 == t2 //\ m" := (Bind_AssertEq_Free _ _ t1 t2 m) (at level 70).
-
-    Fixpoint check (e : expr) : ⊢ʷ Env -> Ty -> FreeM Unit :=
-      fun w G tr =>
-        match e with
-        | v_true => Bind_AssertEq_Free Unit w (Ty_bool w) tr (Ret_Free Unit w tt)
-        | v_false => Bind_AssertEq_Free Unit w (Ty_bool w) tr (Ret_Free Unit w tt)
-        | e_if e0 e1 e2 =>
-          [r1] _ <- check e0 G (Ty_bool w)   ;;
-          [r2] _ <- check e1 G[r1] tr[r1] ;;
-          check e2 G[r1 ⊙ r2] tr[r1 ⊙ r2]
-        | e_var s =>
-          match resolve s G with
-          | Some a => Bind_AssertEq_Free Unit w tr a (Ret_Free Unit w tt)
-          | None => Fail_Free Unit w
+  Definition generate : Exp -> ⊢ʷ Ėnv -> Ṫy -> Free Ėxp :=
+    fix gen e {w} Γ τ :=
+      match e with
+      | exp.var x =>
+          match lookup x Γ with
+          | Some τ' =>
+              [ θ ] _ <- assert τ τ' ;;
+              Ret (ėxp.var x)
+          | None   => Fail
           end
-        | e_absu s e0 =>
-          ∃1, ∃2,
-            let tr' := tr[step ⊙ step] in
-            let α1  := Ty_hole _ 1 (ctx.in_succ ctx.in_zero) in
-            let α2  := Ty_hole _ 2 ctx.in_zero in
-            Ty_func _ α1 α2 == tr' //\
-            check e0 ((s, α1) :: G[step ⊙ step]) α2
+      | exp.true  =>
+          [ θ ] _ <- assert τ ṫy.bool ;;
+          Ret ėxp.true
+      | exp.false =>
+          [ θ ] _ <- assert τ ṫy.bool ;;
+          Ret ėxp.false
+      | exp.ifte e1 e2 e3 =>
+          [ θ1 ] e1' <- gen e1 Γ ṫy.bool ;;
+          [ θ2 ] e2' <- gen e2 Γ[θ1] τ[θ1] ;;
+          [ θ3 ] e3' <- gen e3 Γ[θ1⊙θ2] τ[θ1⊙θ2] ;;
+          Ret (ėxp.ifte e1'[θ2⊙θ3] e2'[θ3] e3')
+      | exp.absu x e =>
+          [ θ1 ] t1  <- choose ;;
+          [ θ2 ] t2  <- choose ;;
+          [ θ3 ] e'  <- gen e (Γ[θ1⊙θ2] ,, x∷t1[θ2]) t2 ;;
+          [ θ4 ] _   <- assert (τ[θ1⊙θ2⊙θ3]) (ṫy.func t1[θ2⊙θ3] t2[θ3]) ;;
+          Ret (ėxp.abst x t1[θ2⊙θ3⊙θ4] e'[θ4])
+      | exp.abst x t1 e =>
+          [ θ1 ] t2  <- choose ;;
+          [ θ2 ] e'  <- gen e (Γ[θ1] ,, x∷lift t1 _) t2 ;;
+          [ θ3 ] _   <- assert (τ[θ1⊙θ2]) (ṫy.func (lift t1 _) t2[θ2]) ;;
+          Ret (ėxp.abst x (lift t1 _) e'[θ3])
+      | exp.app e1 e2 =>
+          [ θ1 ] t1  <- choose ;;
+          [ θ2 ] e1' <- gen e1 Γ[θ1] (ṫy.func t1 τ[θ1]) ;;
+          [ θ3 ] e2' <- gen e2 Γ[θ1⊙θ2] t1[θ2] ;;
+          Ret (ėxp.app e1'[θ3] e2')
+      end.
 
-        | e_abst s t e0 =>
-          ∃2,
-            let tr' := <{ tr ~ step }> in
-            let α1  := lift t (w ▻ 2) in
-            let α2  := Ty_hole (w ▻ 2) 2 ctx.in_zero in
-            Ty_func (w ▻ 2) α1 α2 == tr' //\
-            check e0 ((s, α1) :: <{ G ~ step }>) α2
-        | e_app e0 e1 =>
-          ∃0,
-            let α := Ty_hole (w ▻ 0) 0 ctx.in_zero in
-            [r1] _ <- check e0 <{ G ~ step }> (Ty_func _ α <{ tr ~ step }>) ;;
-                      check e1 G[step ⊙ r1] <{ α ~ r1 }>
+  Definition reconstruct_free (e : Exp) :
+    ⊢ʷ Ėnv -> Free (Prod Ṫy Ėxp) :=
+    fun w G =>
+      [θ1] τ  <- choose ;;
+      [θ2] e' <- generate e G[θ1] τ ;;
+      Ret (τ[θ2] , e').
+
+  Definition reconstruct_optiondiamond (e : Exp) :
+    Option (Diamond alloc.acc_alloc (Ṫy * Sem Exp)) ctx.nil :=
+    option.bind (prenex (reconstruct_free e empty)) solveoptiondiamond.
+
+  Definition reconstruct_schematic (e : Exp) :
+    option (Schematic (Ṫy * Sem Exp)) :=
+    optiondiamond2schematic (reconstruct_optiondiamond e).
+
+  Definition reconstruct_grounded (e : Exp) :
+    option (Ty * Exp) :=
+    option.map
+      (fun s : Schematic _ =>
+         let (w, te) := s in
+         inst te (grounding w))
+      (reconstruct_schematic e).
+
+End Generate.
+
+(* Definition persist_sim_step_alloc_env := Sub.persist_sim_step (Θ := alloc.acc_alloc) (T := Ėnv). *)
+(* Definition persist_sim_step_alloc_ty := Sub.persist_sim_step (Θ := alloc.acc_alloc) (T := Ṫy). *)
+(* Definition persist_sim_step_alloc_sem {A} := Sub.persist_sim_step (Θ := alloc.acc_alloc) (T := Sem A). *)
+
+Ltac wsimpl :=
+  repeat
+    (rewrite ?persist_refl, ?persist_trans, ?persist_lift,
+      ?inst_lift, ?inst_persist, ?inst_refl, ?inst_trans,
+      ?inst_step_snoc, ?lk_trans, ?trans_refl_l, ?trans_refl_r,
+      ?persist_insert, ?lift_insert,
+
+      ?Pred.persist_tpb, ?Pred.persist_and, ?Pred.persist_eq,
+      ?Pred.eqₚ_refl, ?Pred.impl_true_l, ?Pred.and_true_r, ?Pred.and_true_l,
+      ?Pred.impl_true_r, ?Pred.impl_false_l, ?Pred.persist_impl, ?Pred.impl_and,
+      ?Pred.persist_exists, ?Pred.persist_forall, ?Pred.Acc.wlp_true, ?Pred.eq_pair,
+      ?Pred.eq_func,
+
+      (* ?ProgramLogic.eqₚ_env_cons, *)
+      (* ?ProgramLogic.equiv_true, *)
+
+      (* ?persist_sim_step_alloc_env, ?persist_sim_step_alloc_ty, (* ?persist_sim_step_alloc_sem, *) *)
+      ?ėxp.inst_var, ?ėxp.inst_true, ?ėxp.inst_false, ?ėxp.inst_ifte, ?ėxp.inst_absu, ?ėxp.inst_abst, ?ėxp.inst_app,
+      ?Sem.inst_pure, ?Sem.inst_fmap, ?Sem.inst_app, ?Sem.persist_pure, ?Sem.persist_fmap, ?Sem.persist_app in *;
+     cbn - [lk trans step thick]; auto);
+  repeat setoid_rewrite Pred.persist_exists;
+  repeat setoid_rewrite Pred.persist_forall;
+  repeat
+    match goal with
+    | |- context[@persist ?A ?I ?Θ ?w0 ?x ?w1 ?θ] =>
+        is_var x; generalize (@persist A I Θ w0 x w1 θ); clear x; intros x;
+        try (clear w0 θ)
+    | |- context[@lk ?Θ (ctx.snoc ?w0 ?α) ?w1 ?θ ?α ctx.in_zero] =>
+        is_var θ;
+        generalize (@lk Θ (ctx.snoc w0 α) w1 θ α ctx.in_zero);
+        clear θ w0; intros ?t
+    | |- context[fun w : World => Ṫy w] =>
+        change_no_check (fun w : World => Ṫy w) with Ṫy
+    | |- context[fun w : Ctx nat => Sem ?X w] =>
+        change_no_check (fun w : World => Sem X w) with (Sem X)
     end.
 
-  End Check.
+Section Correctness.
 
   Import Pred Pred.notations.
-  Import (hints) Sub.
-  Import ProgramLogic Pred.proofmode.
+  Import Pred.proofmode.
   Import iris.proofmode.tactics.
   Open Scope pred_scope.
 
-  Lemma soundness (e : expr) :
-    forall (w : World) (G : Env w) (tr : Ty w),
-      ⊢ WLP _ (check e G tr) (fun w1 r1 _ => ∃ₚ ee : Expr w1, G[r1] |--ₚ e; tr[r1] ~> ee).
+  Import Pred Pred.notations.
+  Import World.notations.
+  Import (notations) Sem.
+
+  #[local] Arguments Sem.decode_ty : simpl never.
+  #[local] Arguments step : simpl never.
+  (* #[local] Arguments Free.choose : simpl never. *)
+
+  Lemma generate_sound_aux e :
+    forall (w : World) (G : Ėnv w) (t : Ṫy w),
+      ⊢ WLP (Θ := alloc.acc_alloc) (generate e G t) (fun w1 θ ee =>
+                                   G[θ] |--ₚ e; t[θ] ~> ee).
   Proof.
-    induction e; cbn; intros w G tr; unfold T, _4; wsimpl.
-    - constructor. intros ι. pred_unfold.
-      exists (S.pure v_true). constructor.
-    - constructor. intros ι. pred_unfold.
-      exists (S.pure v_false). constructor.
-    - rewrite wlp_bind. unfold _4.
-      iPoseProof (IHe1 w G (Ty_bool w)) as "-#IH1". iRevert "IH1". clear IHe1.
-      iApply wlp_mono. iIntros (w1 r1 _). iIntros "!> [%e1' HT1]".
+    induction e; cbn - [choose]; intros w G τ; unfold T, _4; wsimpl.
+    - destruct lookup eqn:?; wsimpl.
+      constructor. intros ι _; pred_unfold.
+      constructor. now rewrite lookup_inst Heqo.
+    - constructor. intros ι _. pred_unfold. constructor.
+    - constructor. intros ι _. pred_unfold. constructor.
+    - rewrite wlp_bind. unfold _4. cbn.
+      iPoseProof (IHe1 w G ṫy.bool) as "-#IH1". iRevert "IH1". clear IHe1.
+      iApply (@wlp_mono alloc.acc_alloc). iIntros (w1 θ1 e1') "!> HT1".
 
       rewrite wlp_bind. unfold _4.
-      iPoseProof (IHe2 w1 G[r1] tr[r1]) as "-#IH2". iRevert "IH2". clear IHe2.
-      iApply wlp_mono. iIntros (w2 r2 _). iIntros "!> [%e2' HT2]".
+      iPoseProof (IHe2 w1 G[θ1] τ[θ1]) as "-#IH2". iRevert "IH2". clear IHe2.
+      iApply (@wlp_mono alloc.acc_alloc). iIntros (w2 θ2 e2') "!> HT2".
 
-      iPoseProof (IHe3 w2 G[r1 ⊙ r2] tr[r1 ⊙ r2]) as "-#IH3". iRevert "IH3". clear IHe3.
-      iApply wlp_mono. iIntros (w3 r3 _). iIntros "!> [%e3' HT3]".
+      rewrite wlp_bind. unfold _4.
+      iPoseProof (IHe3 w2 G[θ1⊙θ2] τ[θ1⊙θ2]) as "-#IH3". iRevert "IH3". clear IHe3.
+      iApply (@wlp_mono alloc.acc_alloc). iIntros (w3 θ3 e3') "!> HT3". cbn.
       wsimpl.
+      iStopProof. constructor. intros ι (HT1 & HT2 & HT3).
+      pred_unfold. wsimpl. constructor; auto.
 
-      iExists (fun ι => e_if (e1' ι) (e2' ι) (e3' ι)).
-      iStopProof. constructor. intros ι (IH1 & IH2 & IH3). now constructor.
-    - destruct resolve eqn:?; wsimpl.
-      constructor. intros ι; pred_unfold.
-      exists (S.pure (e_var s)).
-      constructor. now rewrite resolve_inst Heqo.
-    - iIntros "!> !> Heq1".
-      iPoseProof (IHe (w ▻ 1 ▻ 2)
-                      ((s, Ty_hole (w ▻ 1 ▻ 2) 1 (ctx.in_succ ctx.in_zero)) :: G[step][step])
-                      (Ty_hole (w ▻ 1 ▻ 2) 2 ctx.in_zero)) as "-#IH". iRevert "IH". clear IHe.
-      iApply wlp_mono. iIntros (w1 r1 _).
-      iIntros "!> [%e' HT]". wsimpl.
-      iExists (fun ι => e_abst s (inst (lk r1 (ctx.in_succ ctx.in_zero)) ι) (e' ι)).
-      iStopProof. constructor. intros ι (Heq & IH). pred_unfold. now constructor.
-    - iIntros "!> Heq".
-      iPoseProof (IHe (w ▻ 2)
-                    ((s, lift t (w ▻ 2)) :: G[step])
-                    (Ty_hole (w ▻ 2) 2 ctx.in_zero))
-                      as "-#IH". iRevert "IH". clear IHe.
-      iApply wlp_mono. iIntros (w1 r1 _).
-      iIntros "!> [%e' HT]". wsimpl.
-      generalize (lk r1 ctx.in_zero). clear w r1. intros t2.
-      iExists (fun ι => e_abst s t (e' ι)).
-      iStopProof. constructor. intros ι (Heq & IH). pred_unfold. now constructor.
-    - iIntros "!>".
+    - iIntros "!> !>".
+      rewrite wlp_bind. unfold _4. cbn.
 
+      iPoseProof (IHe _ (G[step][step] ,, x∷lk step ctx.in_zero) (ṫy.var ctx.in_zero)) as "-#IH". iRevert "IH". clear IHe.
+      iApply (@wlp_mono alloc.acc_alloc). iIntros (w1 θ1 e1').
+      iIntros "!> HT Heq1". rewrite persist_insert. wsimpl.
+      generalize (@lk alloc.acc_alloc (w ▻ @ctx.length nat w)
+                   (w ▻ @ctx.length nat w ▻ S (@ctx.length nat w))
+                   (@step alloc.acc_alloc alloc.step_alloc (w ▻ @ctx.length nat w)
+                      (S (@ctx.length nat w))) (@ctx.length nat w)
+                   (@ctx.in_zero nat (@ctx.length nat w) w))[θ1] as t1.
+      intros t1.
+      generalize (@lk alloc.acc_alloc (w ▻ @ctx.length nat w ▻ S (@ctx.length nat w)) w1 θ1
+                (S (@ctx.length nat w))
+                (@ctx.in_zero nat (S (@ctx.length nat w)) (w ▻ @ctx.length nat w))).
+      intros t2.
+      iStopProof. constructor. intros ι [HT Heq]. pred_unfold.
+      rewrite inst_insert in HT. wsimpl. now constructor.
+    - iIntros "!>". rewrite wlp_bind. unfold _4. cbn.
+      iPoseProof (IHe _ (G[step] ,, x∷lift t (w ▻ ctx.length w)) (ṫy.var ctx.in_zero)) as "-#IH". iRevert "IH". clear IHe.
+      iApply (@wlp_mono alloc.acc_alloc). iIntros (w1 θ1 e1') "!> HT". cbn.
+      rewrite persist_insert. wsimpl.
+      iStopProof. constructor. intros ι HT1. pred_unfold. wsimpl.
+      rewrite inst_insert inst_lift in HT1. now constructor.
+    - iIntros "!>". rewrite wlp_bind. unfold _4.
+      iPoseProof (IHe1 _ G[step] (ṫy.func (ṫy.var ctx.in_zero) τ[step])) as "-#IH". iRevert "IH". clear IHe1.
+      iApply (@wlp_mono alloc.acc_alloc). iIntros (w1 r1 e1') "!> HT1".
       rewrite wlp_bind. unfold _4.
-      iPoseProof (IHe1 (w ▻ 0) G[step] (Ty_func (w ▻ 0) (Ty_hole (w ▻ 0) 0 ctx.in_zero) tr[step]))
-        as "-#IH". iRevert "IH". clear IHe1.
-      iApply wlp_mono. iIntros (w1 r1 _). iIntros "!> [%e1' HT1]".
-
       iPoseProof (IHe2 w1 G[step ⊙ r1] (lk r1 ctx.in_zero)) as "-#IH". iRevert "IH". clear IHe2.
-      iApply wlp_mono. iIntros (w2 r2 _). iIntros "!> [%e2' HT2]". wsimpl.
-      generalize (lk r1 ctx.in_zero)[r2]. clear w r1. intros t1.
-      iExists (fun ι => e_app (e1' ι) (e2' ι)).
-      iStopProof. constructor. intros ι (H1 & H2). pred_unfold.
+      iApply (@wlp_mono alloc.acc_alloc). iIntros (w2 r2 e2') "!> HT2". cbn.
+      wsimpl.
+      iStopProof. constructor. intros ι (HT1 & HT2). pred_unfold. wsimpl.
       econstructor; eauto.
   Qed.
 
-  Lemma completeness_aux {G e t ee} (T : G |-- e; t ~> ee) :
-    forall w0 (G0 : Env w0) (t0 : Ty w0),
-      ⊢ liftEnv G _ =ₚ G0 → lift t _ =ₚ t0 → WP _ (check e G0 t0) (fun _ _ _ => Trueₚ)%P.
+  Definition TPB_algo : ⊢ʷ Ėnv -> Const Exp -> Ṫy -> Ėxp -> Pred :=
+    fun w0 G0 e t0 e0 =>
+    WP (Θ := alloc.acc_alloc)
+      (reconstruct_free e G0)
+      (fun w1 (θ1 : alloc.acc_alloc w0 w1) '(t1,e1) =>
+         t0[θ1] =ₚ t1 /\ₚ
+         e0[θ1] =ₚ e1).
+
+  Lemma generate_sound (e : Exp) (w0 : World) (G0 : Ėnv w0) t0 e0 :
+    TPB_algo G0 e t0 e0 ⊢ₚ G0 |--ₚ e; t0 ~> e0.
   Proof.
-    induction T; intros w0 G0 t0; wsimpl.
-    - iIntros "#HeqG #Heqt". rewrite wp_bind.
-      iPoseProof (IHT1 w0 G0 (Ty_bool w0) with "HeqG") as "-#IHT1".
-      clear IHT1. wsimpl.
-      iRevert "IHT1". iApply wp_mono. iIntros (w1 r1 _). wsimpl.
-      iModIntro. wsimpl. rewrite wp_bind.
-      iPoseProof (IHT2 w1 G0[r1] t0[r1] with "HeqG Heqt") as "-#IHT2".
-      iRevert "IHT2". iApply wp_mono. iIntros (w2 r2 _). wsimpl.
-      iModIntro. wsimpl. unfold _4.
-      iApply IHT3; wsimpl.
-    - constructor. intros ι. intros _ HeqG Heqt. cbn in *.
-      rewrite inst_lift_env in HeqG.
-      rewrite inst_lift in Heqt. subst.
-      rewrite resolve_inst in H.
-      destruct resolve.
-      + injection H. easy.
-      + discriminate H.
-    - iIntros "#HeqG #Heqt".
-      iExists (lift vt _), (lift t _). wsimpl.
-      iSplit. wsimpl.
-      iModIntro. iIntros "#Heq1". iModIntro. iIntros "#Heq2".
-      iPoseProof (IHT (w0 ▻ 1 ▻ 2)
-                    ((v, Ty_hole (w0 ▻ 1 ▻ 2) 1 (ctx.in_succ ctx.in_zero)) :: G0[step][step])
-                    (Ty_hole (w0 ▻ 1 ▻ 2) 2 ctx.in_zero)) as "IHT". clear IHT.
-      wsimpl.
-      iPoseProof ("IHT" with "Heq1 HeqG Heq2") as "-#IHT'". iRevert "IHT'". iClear "IHT".
-      iApply wp_mono. unfold _4. iIntros (w1 r1 _). wsimpl.
-    - iIntros "#HeqG #Heqt".
-      iExists (lift t _). wsimpl.
-      iSplit. wsimpl.
-      iModIntro. iIntros "#Heq1".
-      iPoseProof (IHT (w0 ▻ 2)
-                    ((v, lift vt (w0 ▻ 2)) :: G0[step])
-                    (Ty_hole (w0 ▻ 2) 2 ctx.in_zero)) as "IHT"; clear IHT.
-      wsimpl.
-      iPoseProof ("IHT" with "HeqG Heq1") as "-#IHT'". iRevert "IHT'". iClear "IHT".
-      iApply wp_mono. unfold _4. iIntros (w1 r1 _). wsimpl.
-    - iIntros "#HeqG #Heqt".
-      iExists (lift t2 _).
-      iModIntro. iIntros "#Heq1".
-      rewrite wp_bind.
-      iPoseProof (IHT1 (w0 ▻ 0) G0[step (R := Alloc)] (Ty_func (w0 ▻ 0) (Ty_hole (w0 ▻ 0) 0 ctx.in_zero) t0[step (R := Sub)])) as "IHT1"; clear IHT1.
-      wsimpl.
-      iPoseProof ("IHT1" with "HeqG Heq1 Heqt") as "-#IHT1'". iRevert "IHT1'". iClear "IHT1".
-      iApply wp_mono. unfold _4. iIntros (w1 r1 _). iModIntro. wsimpl.
-      iApply IHT2; wsimpl.
+    iStartProof. rewrite wand_is_impl. rewrite wp_impl. unfold reconstruct_free.
+    rewrite wlp_bind. cbn. unfold _4. iIntros "!>".
+    rewrite wlp_bind. cbn. unfold _4. wsimpl.
+    iPoseProof (@generate_sound_aux e _ G0[step] (ṫy.var ctx.in_zero)) as "-#Hsound".
+    iRevert "Hsound". iApply (@wlp_mono alloc.acc_alloc). iIntros (w1 θ1 e') "!> HT".
+    wsimpl. rewrite <- !persist_trans. wsimpl.
+    iStopProof. constructor. intros ι HT Heqt Heqe. now pred_unfold.
   Qed.
 
-End CandidateType.
+  Lemma generate_complete_aux {G e t ee} (T : G |-- e ∷ t ~> ee) :
+    forall w0 (G0 : Ėnv w0) (t0 : Ṫy w0),
+      ⊢ lift G _ =ₚ G0 ->ₚ
+        lift t _ =ₚ t0 ->ₚ
+      WP (Θ := alloc.acc_alloc) (generate e G0 t0)
+          (fun w1 r01 e' => Sem.pure ee =ₚ e')%P.
+  Proof.
+    induction T as [G x t Hres|G|G|G t e1 e1' e2 e2' e3 e3' _ IH1 _ IH2 _ IH3
+      |G x t1 t2 e e' _ IH|G x t1 t2 e e' _ IH|G e1 t2 e1' e2 t1 e2' _ IH1 _ IH2];
+      intros w0 G0 t0; wsimpl; unfold _4, Worlds.T.
+
+    - constructor. intros ι. unfold eqₚ. pred_unfold.
+      intros _ -> ->.
+      rewrite lookup_inst in Hres.
+      destruct lookup.
+      + injection Hres. now pred_unfold.
+      + discriminate Hres.
+
+    - iIntros "#HeqG #Heqt". cbn. iSplit. rewrite (eqₚ_sym t0). auto.
+      now iApply eqₚ_refl.
+    - iIntros "#HeqG #Heqt". cbn. iSplit. rewrite (eqₚ_sym t0). auto.
+      now iApply eqₚ_refl.
+    - iIntros "#HeqG #Heqt". cbn.
+      rewrite wp_bind. unfold _4.
+      iPoseProof (eqₚ_intro (lift ty.bool w0)) as "Heqbool".
+      iPoseProof (IH1 _ G0 ṫy.bool with "HeqG Heqbool") as "-#IH". clear IH1.
+      iRevert "IH".
+      iApply (@wp_mono alloc.acc_alloc). iIntros (w1 r1 e1'') "!> #Heq1". wsimpl.
+
+      rewrite wp_bind. unfold _4.
+      iPoseProof (IH2 _ G0[r1] t0[r1] with "HeqG Heqt") as "-#IH". clear IH2.
+      iRevert "IH".
+      iApply (@wp_mono alloc.acc_alloc). iIntros (w2 r2 e2'') "!> #Heq2". wsimpl.
+
+      rewrite wp_bind. unfold _4.
+      iPoseProof (IH3 _ G0 t0 with "HeqG Heqt") as "-#IH". clear IH3.
+      iRevert "IH".
+      iApply (@wp_mono alloc.acc_alloc). iIntros (w3 r3 e3'') "!> #Heq3". wsimpl.
+
+      iClear "Heqbool".
+      iStopProof. constructor. intros ι [_ [(HeqG & Heqt & Heq1 & Heq2 & Heq3)]].
+      pred_unfold. wsimpl. now subst.
+
+    - iIntros "#HeqG #Heqt". cbn.
+      rewrite Acc.intro_wp_step.
+      iExists (lift t1 _). iIntros "!> #Heq1".
+      rewrite Acc.intro_wp_step.
+      iExists (lift t2 _). iIntros "!> #Heq2".
+      rewrite wp_bind. unfold _4. wsimpl.
+      iPoseProof (IH _ (G0 ,, x∷lk step ctx.in_zero) (ṫy.var ctx.in_zero)) as "IH".
+      clear IH. wsimpl.
+      rewrite <- eqₚ_insert. wsimpl.
+      iPoseProof ("IH" with "HeqG Heq1 Heq2") as "-#IH'"; iClear "IH". iRevert "IH'".
+      iApply (@wp_mono alloc.acc_alloc).
+      iIntros (w1 r1 e1'') "!> #Heq3". wsimpl.
+      repeat
+        match goal with
+        | |- context[@lk ?Θ (ctx.snoc ?w0 ?α) ?w1 ?θ ?α ctx.in_zero] =>
+            generalize (@lk Θ (ctx.snoc w0 α) w1 θ α ctx.in_zero);
+            intros ?t
+        end.
+      wsimpl.
+      iStopProof. constructor. intros ι [_ [(HeqG & Heqt & Heq1 & Heq2 & Heq3)]].
+      pred_unfold. wsimpl. now subst.
+
+    - iIntros "#HeqG #Heqt". cbn.
+      rewrite Acc.intro_wp_step.
+      iExists (lift t2 _). iIntros "!> #Heq1". wsimpl.
+
+      rewrite wp_bind. unfold _4.
+      iPoseProof (IH _ (G0 ,, x∷lift t1 _) (ṫy.var ctx.in_zero)) as "IH". clear IH. wsimpl.
+      rewrite <- eqₚ_insert. wsimpl.
+      iPoseProof ("IH" with "HeqG Heq1") as "-#IH'"; iClear "IH". iRevert "IH'".
+      iApply (@wp_mono alloc.acc_alloc).
+      iIntros (w1 r1 e'') "!> #Heq2"; wsimpl.
+      iStopProof. constructor. intros ι [_ [(HeqG & Heqt & Heq1 & Heq2)]].
+      pred_unfold. wsimpl. now subst.
+
+    - iIntros "#HeqG #Heqt". cbn.
+      rewrite Acc.intro_wp_step.
+      iExists (lift t1 _). iIntros "!> #Heq1". wsimpl.
+      rewrite wp_bind. unfold _4. wsimpl.
+      iPoseProof (IH1 _ G0[step] (ṫy.func (ṫy.var ctx.in_zero) t0)) as "IH"; clear IH1. wsimpl.
+      iPoseProof ("IH" with "HeqG Heq1 Heqt") as "-#IH'"; iClear "IH". iRevert "IH'".
+      iApply (@wp_mono alloc.acc_alloc).
+      iIntros (w1 r1 e1'') "!> #Heq2"; wsimpl.
+
+      rewrite wp_bind. unfold _4. cbn.
+      iPoseProof (IH2 w1 G0 t with "HeqG Heq1") as "-#IH"; clear IH2. iRevert "IH".
+      iApply (@wp_mono alloc.acc_alloc).
+      iIntros (w2 r2 e2'') "!> #Heq3"; wsimpl.
+
+      iStopProof. constructor. intros ι [_ [(HeqG & Heqt & Heq1 & Heq2 & Heq3)]].
+      pred_unfold. wsimpl. now subst.
+  Qed.
+
+  Lemma generate_complete (e : Exp) (w0 : World) (G0 : Ėnv w0) t0 e0 :
+    G0 |--ₚ e; t0 ~> e0 ⊢ₚ TPB_algo G0 e t0 e0.
+  Proof.
+    iIntros "HT". unfold TPB_algo, reconstruct_free. rewrite wp_bind. cbn. unfold _4.
+    rewrite Acc.intro_wp_step.
+    iExists t0. iIntros "!> Heq1". wsimpl.
+    rewrite wp_bind. unfold _4. cbn.
+    iStopProof. constructor. intros ι [HT Heq]. pred_unfold.
+    pose proof (@generate_complete_aux _ _ _ _ HT _ G0 (ṫy.var ctx.in_zero)) as [Hcompl].
+    specialize (Hcompl ι (MkEmp _)). pred_unfold.
+    specialize (Hcompl eq_refl Heq). revert Hcompl.
+    apply wp_mono. intros w1 θ1 e1.
+    wsimpl. intros ι1 <-. pred_unfold. wsimpl.
+  Qed.
+
+  Lemma generate_correct (e : Exp) (w0 : World) (G0 : Ėnv w0) t0 e0 :
+    G0 |--ₚ e; t0 ~> e0 ⊣⊢ₚ TPB_algo G0 e t0 e0.
+  Proof. apply split_bientails. auto using generate_complete, generate_sound. Qed.
+
+  Import (hints) Triangular.Tri.
+  Import (hints) Acc.
+
+  Definition TPB_OD (e : Exp) (t : Ty) (ee : Exp) : Pred ctx.nil :=
+    wp_optiondiamond (reconstruct_optiondiamond e)
+      (fun w θ '(t', ee') => t' =ₚ lift t w /\ₚ ee' =ₚ lift ee w).
+
+  Lemma proper_wp_option_bientails {A : TYPE} {w1 w2: World} (m : Option A w1) :
+    Proper (pointwise_relation (A w1) bientails ==> bientails) (@wp_option A w1 w2 m).
+  Proof.
+    intros P Q PQ. unfold pointwise_relation in PQ.
+    destruct m; cbn; easy.
+  Qed.
+
+  Lemma reconstruct_schematic_correct (e : Exp) t ee :
+    ∅ |--ₚ e; lift t _ ~> lift ee _ ⊣⊢ₚ TPB_OD e t ee.
+  Proof.
+    rewrite generate_correct. unfold TPB_algo, TPB_OD, reconstruct_free.
+    rewrite wp_bind. unfold reconstruct_optiondiamond.
+    rewrite wp_optiondiamond_bind'.
+    unfold reconstruct_free. cbn.
+    rewrite wp_option_bind. unfold T, _4.
+    wsimpl.
+    rewrite <- prenex_correct.
+    generalize
+(@prenex (Prod Ṫy (Sem Exp)) (@ctx.snoc nat (@ctx.nil nat) 0)
+             (@bind alloc.acc_alloc Free
+                (@bind_freem alloc.acc_alloc alloc.refl_alloc alloc.trans_alloc
+                   alloc.step_alloc) (Sem Exp) (Prod Ṫy (Sem Exp))
+                (@ctx.snoc nat (@ctx.nil nat) 0)
+                (@generate e (@ctx.snoc nat (@ctx.nil nat) 0)
+                   (@persist Ėnv persist_env alloc.acc_alloc (@ctx.nil nat)
+                      (@empty (Ėnv (@ctx.nil nat))
+                         (@gmap_empty string string_eq_dec string_countable
+                            (Ṫy (@ctx.nil nat)))) (@ctx.snoc nat (@ctx.nil nat) 0)
+                      (@step alloc.acc_alloc alloc.step_alloc (@ctx.nil nat) 0))
+                   (@ṫy.var (@ctx.snoc nat (@ctx.nil nat) 0) 0
+                      (@ctx.in_zero nat 0 (@ctx.nil nat))))
+                (fun (w1 : Ctx nat)
+                   (θ2 : alloc.acc_alloc (@ctx.snoc nat (@ctx.nil nat) 0) w1)
+                   (e' : Sem Exp w1) =>
+                 @Ret (Prod Ṫy (Sem Exp)) w1
+                   (@pair (Ṫy w1) (Sem Exp w1)
+                      (@lk alloc.acc_alloc (@ctx.snoc nat (@ctx.nil nat) 0) w1 θ2 0
+                         (@ctx.in_zero nat 0 (@ctx.nil nat))) e')))).
+    intros m.
+    unfold wp_prenex, wp_optiondiamond. cbn.
+    unfold _4. cbn.
+    destruct m as [(w1 & θ1 & C & t' & ee')|]; cbn; [|now rewrite Acc.wp_false].
+    cbn. wsimpl.
+    rewrite wp_option_bind.
+    rewrite <- solvelist_correct.
+    destruct (solvelist C) as [(w2 & θ2 & [])|]; cbn.
+    - rewrite Acc.and_wp_l. wsimpl. clear.
+      rewrite eqₚ_sym.
+      generalize (t' =ₚ lift t w2). clear. intros P.
+      rewrite eqₚ_sym.
+      generalize (P /\ₚ ee' =ₚ lift ee w2). clear. intros P.
+      constructor; intros ι.
+      destruct (env.view ι). cbn.
+      split; intros [ι]; firstorder.
+      exists (env.snoc env.nil _ (inst (lk θ1 ctx.in_zero) (inst θ2 ι))).
+      split; auto.
+      exists (inst θ2 ι). firstorder.
+    - now rewrite and_false_l !Acc.wp_false.
+  Qed.
+
+  Definition tpb_algo (e : Exp) (t : Ty) (ee : Exp) : Prop :=
+    match reconstruct_schematic e with
+    | Some (existT w (t', ee')) =>
+        exists ι : Assignment w, inst t' ι = t /\ inst ee' ι = ee
+    | None => False
+    end.
+
+  Lemma correctness (e : Exp) (t : Ty) (ee : Exp) :
+    tpb empty e t ee <-> tpb_algo e t ee.
+  Proof.
+    generalize (reconstruct_schematic_correct e t ee).
+    unfold TPB_OD, tpb_algo, reconstruct_schematic.
+    intros [HE]. specialize (HE env.nil). pred_unfold.
+    rewrite inst_empty in HE. rewrite HE. clear HE.
+    destruct reconstruct_optiondiamond as [(w & θ & [t' ee'])|]; cbn; auto.
+    apply base.exist_proper. intros ι. pred_unfold. intuition.
+  Qed.
+
+  Print Assumptions correctness.
+
+End Correctness.
